backend/Allocproof.v
@@ -1786,30 +1786,41 @@ Variable prog: RTL.program.
 Variable tprog: LTL.program.
 Hypothesis TRANSF: match_prog prog tprog.
 
-Let ge := Genv.globalenv prog.
-Let tge := Genv.globalenv tprog.
+Ltac UseShape :=
+  match goal with
+  | [ WT: wt_function _ _, CODE: (RTL.fn_code _)!_ = Some _, EQ: transfer _ _ _ _ _ = OK _ |- _ ] =>
+      destruct (invert_code _ _ _ _ _ _ _ WT CODE EQ) as (eafter & bsh & bb & AFTER & BSH & TCODE & EBS & TR & WTI);
+      inv EBS; unfold transfer_aux in TR; MonadInv
+  end.
+
+Section CORELEMMA.
+
+Variable ge : RTL.genv.
+Variable tge : genv.
+
+Hypothesis (MATCH_GENV: Genv.match_genvs (match_globdef (fun _ f tf => transf_fundef f = OK tf) eq prog) ge tge).
 
 Lemma symbols_preserved:
   forall (s: ident), Genv.find_symbol tge s = Genv.find_symbol ge s.
-Proof (Genv.find_symbol_match TRANSF).
+Proof (Genv.find_symbol_match_genv MATCH_GENV).
 
 Lemma senv_preserved:
   Senv.equiv ge tge.
-Proof (Genv.senv_match TRANSF).
+Proof (Genv.senv_match_genv MATCH_GENV).
 
 Lemma functions_translated:
   forall (v: val) (f: RTL.fundef),
   Genv.find_funct ge v = Some f ->
   exists tf,
   Genv.find_funct tge v = Some tf /\ transf_fundef f = OK tf.
-Proof (Genv.find_funct_transf_partial TRANSF).
+Proof (Genv.find_funct_transf_partial_genv MATCH_GENV).
 
 Lemma function_ptr_translated:
   forall (b: block) (f: RTL.fundef),
   Genv.find_funct_ptr ge b = Some f ->
   exists tf,
   Genv.find_funct_ptr tge b = Some tf /\ transf_fundef f = OK tf.
-Proof (Genv.find_funct_ptr_transf_partial TRANSF).
+Proof (Genv.find_funct_ptr_transf_partial_genv MATCH_GENV).
 
 Lemma sig_function_translated:
   forall f tf,
@@ -1961,13 +1972,6 @@ Proof.
   unfold proj_sig_res in *. rewrite H0; auto.
   intros. rewrite (loc_result_exten sg' sg) in H by auto. eauto.
 Qed.
-
-Ltac UseShape :=
-  match goal with
-  | [ WT: wt_function _ _, CODE: (RTL.fn_code _)!_ = Some _, EQ: transfer _ _ _ _ _ = OK _ |- _ ] =>
-      destruct (invert_code _ _ _ _ _ _ _ WT CODE EQ) as (eafter & bsh & bb & AFTER & BSH & TCODE & EBS & TR & WTI);
-      inv EBS; unfold transfer_aux in TR; MonadInv
-  end.
 
 Remark addressing_not_long:
   forall env f addr args dst s r,
@@ -2122,7 +2126,6 @@ Proof.
   { replace (rs##args) with ((rs#dst<-v)##args).
     eapply add_equations_lessdef; eauto.
     apply list_map_exten; intros. rewrite Regmap.gso; auto.
-    eapply addressing_not_long; eauto.
   }
   exploit eval_addressing_lessdef. eexact LD3.
   eapply eval_offset_addressing; eauto; apply Archi.splitlong_ptr32; auto.
@@ -2482,9 +2485,19 @@ Proof.
   apply wt_regset_assign; auto. rewrite WTRES0; auto.
 Qed.
 
+End CORELEMMA.
+
+Section WHOLE.
+
+Let ge := Genv.globalenv prog.
+Let tge := Genv.globalenv tprog.
+
+Let MATCH_GENV: Genv.match_genvs (match_globdef (fun _ f tf => transf_fundef f = OK tf) eq prog) ge tge.
+Proof. apply Genv.globalenvs_match; eauto. Qed.
+
 Lemma initial_states_simulation:
   forall st1, RTL.initial_state prog st1 ->
-  exists st2, LTL.initial_state tprog st2 /\ match_states st1 st2.
+  exists st2, LTL.initial_state tprog st2 /\ match_states tge st1 st2.
 Proof.
   intros. inv H.
   exploit function_ptr_translated; eauto. intros [tf [FIND TR]].
@@ -2492,7 +2505,7 @@ Proof.
   exists (LTL.Callstate nil tf (Locmap.init Vundef) m0); split.
   econstructor; eauto.
   eapply (Genv.init_mem_transf_partial TRANSF); eauto.
-  rewrite symbols_preserved.
+  erewrite symbols_preserved; eauto.
   rewrite (match_program_main TRANSF).  auto.
   congruence.
   constructor; auto.
@@ -2505,7 +2518,7 @@ Qed.
 
 Lemma final_states_simulation:
   forall st1 st2 r,
-  match_states st1 st2 -> RTL.final_state st1 r -> LTL.final_state st2 r.
+  match_states tge st1 st2 -> RTL.final_state st1 r -> LTL.final_state st2 r.
 Proof.
   intros. inv H0. inv H. inv STACKS.
   econstructor. rewrite <- (loc_result_exten sg). inv RES; auto.
@@ -2528,9 +2541,9 @@ Qed.
 Theorem transf_program_correct:
   forward_simulation (RTL.semantics prog) (LTL.semantics tprog).
 Proof.
-  set (ms := fun s s' => wt_state s /\ match_states s s').
+  set (ms := fun s s' => wt_state s /\ match_states tge s s').
   eapply forward_simulation_plus with (match_states := ms).
-- apply senv_preserved.
+- apply senv_preserved; auto.
 - intros. exploit initial_states_simulation; eauto. intros [st2 [A B]].
   exists st2; split; auto. split; auto.
   apply wt_initial_state with (p := prog); auto. exact wt_prog.
@@ -2541,5 +2554,7 @@ Proof.
   eapply subject_reduction; eauto. eexact wt_prog. eexact H.
   auto.
 Qed.
+
+End WHOLE.
 
 End PRESERVATION.
