backend/CleanupLabelsproof.v
@@ -34,29 +34,34 @@ Section CLEANUP.
 
 Variables prog tprog: program.
 Hypothesis TRANSL: match_prog prog tprog.
-Let ge := Genv.globalenv prog.
-Let tge := Genv.globalenv tprog.
+
+Section CORELEMMA.
+
+Variable ge : genv.
+Variable tge : genv.
+
+Hypothesis (MATCH_GENV: Genv.match_genvs (match_globdef (fun ctx f tf => tf = transf_fundef f) eq prog) ge tge).
 
 Lemma symbols_preserved:
   forall id,
   Genv.find_symbol tge id = Genv.find_symbol ge id.
-Proof (Genv.find_symbol_transf TRANSL).
+Proof (Genv.find_symbol_transf_genv MATCH_GENV).
 
 Lemma senv_preserved:
   Senv.equiv ge tge.
-Proof (Genv.senv_transf TRANSL).
+Proof (Genv.senv_transf_genv MATCH_GENV).
 
 Lemma functions_translated:
   forall v f,
   Genv.find_funct ge v = Some f ->
   Genv.find_funct tge v = Some (transf_fundef f).
-Proof (Genv.find_funct_transf TRANSL).
+Proof (Genv.find_funct_transf_genv MATCH_GENV).
 
 Lemma function_ptr_translated:
   forall v f,
   Genv.find_funct_ptr ge v = Some f ->
   Genv.find_funct_ptr tge v = Some (transf_fundef f).
-Proof (Genv.find_funct_ptr_transf TRANSL).
+Proof (Genv.find_funct_ptr_transf_genv MATCH_GENV).
 
 Lemma sig_function_translated:
   forall f,
@@ -323,6 +328,16 @@ Proof.
   econstructor; eauto.
 Qed.
 
+End CORELEMMA.
+
+Section WHOLE.
+
+Let ge := Genv.globalenv prog.
+Let tge := Genv.globalenv tprog.
+
+Let MATCH_GENV: Genv.match_genvs (match_globdef (fun ctx f tf => tf = transf_fundef f) eq prog) ge tge.
+Proof. apply Genv.globalenvs_match; auto. Qed.
+
 Lemma transf_initial_states:
   forall st1, initial_state prog st1 ->
   exists st2, initial_state tprog st2 /\ match_states st1 st2.
@@ -331,8 +346,8 @@ Proof.
   econstructor; split.
   eapply initial_state_intro with (f := transf_fundef f).
   eapply (Genv.init_mem_transf TRANSL); eauto.
-  rewrite (match_program_main TRANSL), symbols_preserved; eauto.
-  apply function_ptr_translated; auto.
+  erewrite (match_program_main TRANSL), symbols_preserved; eauto.
+  eapply function_ptr_translated; eauto.
   rewrite sig_function_translated. auto.
   constructor; auto. constructor.
 Qed.
@@ -348,11 +363,12 @@ Theorem transf_program_correct:
   forward_simulation (Linear.semantics prog) (Linear.semantics tprog).
 Proof.
   eapply forward_simulation_opt.
-  apply senv_preserved.
+  apply senv_preserved; auto.
   eexact transf_initial_states.
   eexact transf_final_states.
-  eexact transf_step_correct.
+  apply transf_step_correct; auto.
 Qed.
 
-End CLEANUP.
+End WHOLE.
 
+End CLEANUP.
