backend/Deadcodeproof.v
@@ -383,30 +383,35 @@ Section PRESERVATION.
 Variable prog: program.
 Variable tprog: program.
 Hypothesis TRANSF: match_prog prog tprog.
-Let ge := Genv.globalenv prog.
-Let tge := Genv.globalenv tprog.
+
+Section CORELEMMA.
+
+Variable ge : genv.
+Variable tge : genv.
+
+Hypothesis (MATCH_GENV: Genv.match_genvs (match_globdef (fun cu f tf => transf_fundef (romem_for cu) f = OK tf) eq prog) ge tge).
 
 Lemma symbols_preserved:
   forall (s: ident), Genv.find_symbol tge s = Genv.find_symbol ge s.
-Proof (Genv.find_symbol_match TRANSF).
+Proof (Genv.find_symbol_match_genv MATCH_GENV).
 
 Lemma senv_preserved:
   Senv.equiv ge tge.
-Proof (Genv.senv_match TRANSF).
+Proof (Genv.senv_match_genv MATCH_GENV).
 
 Lemma functions_translated:
   forall (v: val) (f: RTL.fundef),
   Genv.find_funct ge v = Some f ->
   exists cu tf,
   Genv.find_funct tge v = Some tf /\ transf_fundef (romem_for cu) f = OK tf /\ linkorder cu prog.
-Proof (Genv.find_funct_match TRANSF).
+Proof (Genv.find_funct_match_genv MATCH_GENV).
 
 Lemma function_ptr_translated:
   forall (b: block) (f: RTL.fundef),
   Genv.find_funct_ptr ge b = Some f ->
   exists cu tf,
   Genv.find_funct_ptr tge b = Some tf /\ transf_fundef (romem_for cu) f = OK tf /\ linkorder cu prog.
-Proof (Genv.find_funct_ptr_match TRANSF).
+Proof (Genv.find_funct_ptr_match_genv MATCH_GENV).
 
 Lemma sig_function_translated:
   forall rm f tf,
@@ -717,7 +722,7 @@ Qed.
 
 Theorem step_simulation:
   forall S1 t S2, step ge S1 t S2 ->
-  forall S1', match_states S1 S1' -> sound_state prog S1 ->
+  forall S1', match_states S1 S1' -> sound_state prog ge S1 ->
   exists S2', step tge S1' t S2' /\ match_states S2 S2'.
 Proof.
 
@@ -1106,9 +1111,19 @@ Ltac UseTransfer :=
   econstructor; eauto. apply mextends_agree; auto.
 Qed.
 
+End CORELEMMA.
+
+Section WHOLE.
+
+Let ge := Genv.globalenv prog.
+Let tge := Genv.globalenv tprog.
+
+Let MATCH_GENV: Genv.match_genvs (match_globdef (fun cu f tf => transf_fundef (romem_for cu) f = OK tf) eq prog) ge tge.
+Proof. apply Genv.globalenvs_match; auto. Qed.
+
 Lemma transf_initial_states:
   forall st1, initial_state prog st1 ->
-  exists st2, initial_state tprog st2 /\ match_states st1 st2.
+  exists st2, initial_state tprog st2 /\ match_states ge st1 st2.
 Proof.
   intros. inversion H.
   exploit function_ptr_translated; eauto. intros (cu & tf & A & B & C).
@@ -1116,7 +1131,7 @@ Proof.
   econstructor; eauto.
   eapply (Genv.init_mem_match TRANSF); eauto.
   replace (prog_main tprog) with (prog_main prog).
-  rewrite symbols_preserved. eauto.
+  erewrite symbols_preserved; eauto.
   symmetry; eapply match_program_main; eauto.
   rewrite <- H3. eapply sig_function_translated; eauto.
   econstructor; eauto. constructor. apply Mem.extends_refl.
@@ -1124,7 +1139,7 @@ Qed.
 
 Lemma transf_final_states:
   forall st1 st2 r,
-  match_states st1 st2 -> final_state st1 r -> final_state st2 r.
+  match_states ge st1 st2 -> final_state st1 r -> final_state st2 r.
 Proof.
   intros. inv H0. inv H. inv STACKS. inv RES. constructor.
 Qed.
@@ -1136,15 +1151,17 @@ Theorem transf_program_correct:
 Proof.
   intros.
   apply forward_simulation_step with
-     (match_states := fun s1 s2 => sound_state prog s1 /\ match_states s1 s2).
-- apply senv_preserved.
+     (match_states := fun s1 s2 => sound_state prog ge s1 /\ match_states ge s1 s2).
+- apply senv_preserved; auto.
 - simpl; intros. exploit transf_initial_states; eauto. intros [st2 [A B]].
   exists st2; intuition. eapply sound_initial; eauto.
 - simpl; intros. destruct H. eapply transf_final_states; eauto.
 - simpl; intros. destruct H0.
-  assert (sound_state prog s1') by (eapply sound_step; eauto).
+  assert (sound_state prog ge s1') by (eapply sound_step; eauto).
   fold ge; fold tge. exploit step_simulation; eauto. intros [st2' [A B]].
   exists st2'; auto.
 Qed.
+
+End WHOLE.
 
 End PRESERVATION.
