backend/Debugvarproof.v
@@ -291,30 +291,34 @@ Variable tprog: program.
 
 Hypothesis TRANSF: match_prog prog tprog.
 
-Let ge := Genv.globalenv prog.
-Let tge := Genv.globalenv tprog.
+Section CORELEMMA.
+
+Variable ge : genv.
+Variable tge : genv.
+
+Hypothesis (MATCH_GENV: Genv.match_genvs (match_globdef (fun _ f tf => transf_fundef f = OK tf) eq prog) ge tge).
 
 Lemma symbols_preserved:
   forall (s: ident), Genv.find_symbol tge s = Genv.find_symbol ge s.
-Proof (Genv.find_symbol_match TRANSF).
+Proof (Genv.find_symbol_match_genv MATCH_GENV).
 
 Lemma senv_preserved:
   Senv.equiv ge tge.
-Proof (Genv.senv_match TRANSF).
+Proof (Genv.senv_match_genv MATCH_GENV).
 
 Lemma functions_translated:
   forall (v: val) (f: fundef),
   Genv.find_funct ge v = Some f ->
   exists tf,
   Genv.find_funct tge v = Some tf /\ transf_fundef f = OK tf.
-Proof (Genv.find_funct_transf_partial TRANSF).
+Proof (Genv.find_funct_transf_partial_genv MATCH_GENV).
 
 Lemma function_ptr_translated:
   forall (b: block) (f: fundef),
   Genv.find_funct_ptr ge b = Some f ->
   exists tf,
   Genv.find_funct_ptr tge b = Some tf /\ transf_fundef f = OK tf.
-Proof (Genv.find_funct_ptr_transf_partial TRANSF).
+Proof (Genv.find_funct_ptr_transf_partial_genv MATCH_GENV).
 
 Lemma sig_preserved:
   forall f tf,
@@ -527,6 +531,16 @@ Proof.
   constructor; auto.
 Qed.
 
+End CORELEMMA.
+
+Section WHOLE.
+
+Let ge := Genv.globalenv prog.
+Let tge := Genv.globalenv tprog.
+
+Let MATCH_GENV: Genv.match_genvs (match_globdef (fun _ f tf => transf_fundef f = OK tf) eq prog) ge tge.
+Proof. apply Genv.globalenvs_match; auto. Qed.
+
 Lemma transf_initial_states:
   forall st1, initial_state prog st1 ->
   exists st2, initial_state tprog st2 /\ match_states st1 st2.
@@ -535,7 +549,7 @@ Proof.
   exploit function_ptr_translated; eauto. intros [tf [A B]].
   exists (Callstate nil tf (Locmap.init Vundef) m0); split.
   econstructor; eauto. eapply (Genv.init_mem_transf_partial TRANSF); eauto.
-  rewrite (match_program_main TRANSF), symbols_preserved. auto.
+  erewrite (match_program_main TRANSF), symbols_preserved; eauto.
   rewrite <- H3. apply sig_preserved. auto.
   constructor. constructor. auto.
 Qed.
@@ -551,10 +565,12 @@ Theorem transf_program_correct:
   forward_simulation (semantics prog) (semantics tprog).
 Proof.
   eapply forward_simulation_plus.
-  apply senv_preserved.
+  apply senv_preserved; auto.
   eexact transf_initial_states.
   eexact transf_final_states.
-  eexact transf_step_correct.
+  apply transf_step_correct; auto.
 Qed.
+
+End WHOLE.
 
 End PRESERVATION.
