lib/Coqlib.v
@@ -22,6 +22,7 @@ Require Export ZArith.
 Require Export Znumtheory.
 Require Export List.
 Require Export Bool.
+From Paco Require Export paco.
 
 Global Set Asymmetric Patterns.
 
