x86/Asmgenproof.v
@@ -33,23 +33,28 @@ Section PRESERVATION.
 Variable prog: Mach.program.
 Variable tprog: Asm.program.
 Hypothesis TRANSF: match_prog prog tprog.
-Let ge := Genv.globalenv prog.
-Let tge := Genv.globalenv tprog.
+
+Section CORELEMMA.
+
+Variable ge : Mach.genv.
+Variable tge : Asm.genv.
+
+Hypothesis (MATCH_GENV: Genv.match_genvs (match_globdef (fun _ f tf => transf_fundef f = OK tf) eq prog) ge tge).
 
 Lemma symbols_preserved:
   forall (s: ident), Genv.find_symbol tge s = Genv.find_symbol ge s.
-Proof (Genv.find_symbol_match TRANSF).
+Proof (Genv.find_symbol_match_genv MATCH_GENV).
 
 Lemma senv_preserved:
   Senv.equiv ge tge.
-Proof (Genv.senv_match TRANSF).
+Proof (Genv.senv_match_genv MATCH_GENV).
 
 Lemma functions_translated:
   forall b f,
   Genv.find_funct_ptr ge b = Some f ->
   exists tf,
   Genv.find_funct_ptr tge b = Some tf /\ transf_fundef f = OK tf.
-Proof (Genv.find_funct_ptr_transf_partial TRANSF).
+Proof (Genv.find_funct_ptr_transf_partial_genv MATCH_GENV).
 
 Lemma functions_transl:
   forall fb f tf,
@@ -878,9 +883,19 @@ Transparent destroyed_at_function_entry.
   econstructor; eauto. rewrite ATPC; eauto. congruence.
 Qed.
 
+End CORELEMMA.
+
+Section WHOLE.
+
+Let ge := Genv.globalenv prog.
+Let tge := Genv.globalenv tprog.
+
+Let MATCH_GENV: Genv.match_genvs (match_globdef (fun _ f tf => transf_fundef f = OK tf) eq prog) ge tge.
+Proof. apply Genv.globalenvs_match; auto. Qed.
+
 Lemma transf_initial_states:
   forall st1, Mach.initial_state prog st1 ->
-  exists st2, Asm.initial_state tprog st2 /\ match_states st1 st2.
+  exists st2, Asm.initial_state tprog st2 /\ match_states ge st1 st2.
 Proof.
   intros. inversion H. unfold ge0 in *.
   econstructor; split.
@@ -896,13 +911,13 @@ Proof.
   intros. rewrite Regmap.gi. auto.
   unfold Genv.symbol_address.
   rewrite (match_program_main TRANSF).
-  rewrite symbols_preserved.
+  erewrite symbols_preserved; eauto.
   unfold ge; rewrite H1. auto.
 Qed.
 
 Lemma transf_final_states:
   forall st1 st2 r,
-  match_states st1 st2 -> Mach.final_state st1 r -> Asm.final_state st2 r.
+  match_states ge st1 st2 -> Mach.final_state st1 r -> Asm.final_state st2 r.
 Proof.
   intros. inv H0. inv H. constructor. auto.
   assert (r0 = AX).
@@ -915,10 +930,12 @@ Theorem transf_program_correct:
   forward_simulation (Mach.semantics return_address_offset prog) (Asm.semantics tprog).
 Proof.
   eapply forward_simulation_star with (measure := measure).
-  apply senv_preserved.
+  apply senv_preserved; auto.
   eexact transf_initial_states.
   eexact transf_final_states.
-  exact step_simulation.
+  apply step_simulation; auto.
 Qed.
+
+End WHOLE.
 
 End PRESERVATION.
