x86/SelectLongproof.v
@@ -29,10 +29,12 @@ Section CMCONSTR.
 Variable prog: program.
 Variable hf: helper_functions.
 Hypothesis HELPERS: helper_functions_declared prog hf.
-Let ge := Genv.globalenv prog.
+Variable ge : genv.
 Variable sp: val.
 Variable e: env.
 Variable m: mem.
+
+Hypothesis (GENV_COMPAT: genv_compat ge prog).
 
 Definition unary_constructor_sound (cstr: expr -> expr) (sem: val -> val) : Prop :=
   forall le a x,
@@ -204,7 +206,7 @@ Qed.
 
 Theorem eval_shllimm: forall n, unary_constructor_sound (fun e => shllimm e n) (fun v => Val.shll v (Vint n)).
 Proof.
-  intros; unfold shllimm. destruct Archi.splitlong eqn:SL. apply SplitLongproof.eval_shllimm; auto.
+  intros; unfold shllimm. destruct Archi.splitlong eqn:SL. eapply SplitLongproof.eval_shllimm; eauto.
   red; intros.
   predSpec Int.eq Int.eq_spec n Int.zero.
   exists x; split; auto. subst n; destruct x; simpl; auto.
@@ -233,7 +235,7 @@ Qed.
 
 Theorem eval_shrluimm: forall n, unary_constructor_sound (fun e => shrluimm e n) (fun v => Val.shrlu v (Vint n)).
 Proof.
-  intros; unfold shrluimm. destruct Archi.splitlong eqn:SL. apply SplitLongproof.eval_shrluimm; auto.
+  intros; unfold shrluimm. destruct Archi.splitlong eqn:SL. eapply SplitLongproof.eval_shrluimm; eauto.
   red; intros.
   predSpec Int.eq Int.eq_spec n Int.zero.
   exists x; split; auto. subst n; destruct x; simpl; auto.
@@ -255,7 +257,7 @@ Qed.
 
 Theorem eval_shrlimm: forall n, unary_constructor_sound (fun e => shrlimm e n) (fun v => Val.shrl v (Vint n)).
 Proof.
-  intros; unfold shrlimm. destruct Archi.splitlong eqn:SL. apply SplitLongproof.eval_shrlimm; auto.
+  intros; unfold shrlimm. destruct Archi.splitlong eqn:SL. eapply SplitLongproof.eval_shrlimm; eauto.
   red; intros.
   predSpec Int.eq Int.eq_spec n Int.zero.
   exists x; split; auto. subst n; destruct x; simpl; auto.
@@ -277,7 +279,7 @@ Qed.
 
 Theorem eval_shll: binary_constructor_sound shll Val.shll.
 Proof.
-  unfold shll. destruct Archi.splitlong eqn:SL. apply SplitLongproof.eval_shll; auto.
+  unfold shll. destruct Archi.splitlong eqn:SL. eapply SplitLongproof.eval_shll; eauto.
   red; intros. destruct (is_intconst b) as [n2|] eqn:C.
 - exploit is_intconst_sound; eauto. intros EQ; subst y. apply eval_shllimm; auto.
 - TrivialExists.
@@ -285,7 +287,7 @@ Qed.
 
 Theorem eval_shrlu: binary_constructor_sound shrlu Val.shrlu.
 Proof.
-  unfold shrlu. destruct Archi.splitlong eqn:SL. apply SplitLongproof.eval_shrlu; auto.
+  unfold shrlu. destruct Archi.splitlong eqn:SL. eapply SplitLongproof.eval_shrlu; eauto.
   red; intros. destruct (is_intconst b) as [n2|] eqn:C.
 - exploit is_intconst_sound; eauto. intros EQ; subst y. apply eval_shrluimm; auto.
 - TrivialExists.
@@ -293,7 +295,7 @@ Qed.
 
 Theorem eval_shrl: binary_constructor_sound shrl Val.shrl.
 Proof.
-  unfold shrl. destruct Archi.splitlong eqn:SL. apply SplitLongproof.eval_shrl; auto.
+  unfold shrl. destruct Archi.splitlong eqn:SL. eapply SplitLongproof.eval_shrl; eauto.
   red; intros. destruct (is_intconst b) as [n2|] eqn:C.
 - exploit is_intconst_sound; eauto. intros EQ; subst y. apply eval_shrlimm; auto.
 - TrivialExists.
@@ -419,7 +421,7 @@ Qed.
 
 Theorem eval_mull: binary_constructor_sound mull Val.mull.
 Proof.
-  unfold mull. destruct Archi.splitlong eqn:SL. apply SplitLongproof.eval_mull; auto.
+  unfold mull. destruct Archi.splitlong eqn:SL. eapply SplitLongproof.eval_mull; eauto.
   red; intros; destruct (mull_match a b); InvEval.
 - rewrite Val.mull_commut. apply eval_mullimm; auto.
 - apply eval_mullimm; auto.
@@ -429,14 +431,14 @@ Qed.
 Theorem eval_mullhu:
   forall n, unary_constructor_sound (fun a => mullhu a n) (fun v => Val.mullhu v (Vlong n)).
 Proof.
-  unfold mullhu; intros. destruct Archi.splitlong eqn:SL. apply SplitLongproof.eval_mullhu; auto.
+  unfold mullhu; intros. destruct Archi.splitlong eqn:SL. eapply SplitLongproof.eval_mullhu; eauto.
   red; intros. TrivialExists. constructor. eauto. constructor. apply eval_longconst. constructor. auto.
 Qed.
 
 Theorem eval_mullhs:
   forall n, unary_constructor_sound (fun a => mullhs a n) (fun v => Val.mullhs v (Vlong n)).
 Proof.
-  unfold mullhs; intros. destruct Archi.splitlong eqn:SL. apply SplitLongproof.eval_mullhs; auto.
+  unfold mullhs; intros. destruct Archi.splitlong eqn:SL. eapply SplitLongproof.eval_mullhs; eauto.
   red; intros. TrivialExists. constructor. eauto. constructor. apply eval_longconst. constructor. auto.
 Qed.
 
